examples/acl2/ml/load_defaxioms.ml
@@ -1,8 +1,61 @@
 (*****************************************************************************)
-(* Slurp in defaxioms.lisp.trans.ml                                          *)
+(* Slurp in defaxioms.lisp.trans.ml and put results on variable defaxioms.   *)
 (*****************************************************************************)
 
+new_theory "defaxioms";
+
+quietdec := true;
 use (Globals.HOLDIR ^ "/examples/acl2/ml/load_sexp.ml");
 use (Globals.HOLDIR ^ "/examples/acl2/lisp/defaxioms.lisp.trans.ml");
 load_defaxioms();
+val string_abbrev_thms = map snd (definitions "-");
+quietdec := false;
+
+val List_def =
+ Define
+  `(List[] = nil)
+    /\
+    (List(s::sl) = cons s (List sl))`;
+
+val acl2_and_def =
+ Define
+  `acl2_and x y = ite x y (List[])`;
+
+val acl2_and_def =
+ Define
+  `(acl2_and[] = nil)
+   /\
+   (acl2_and((test,val)::sl) = ite test val (acl2_and sl))`;
+
+val asym_def = Define `asym = sym ACL2`;
+val csym_def = Define `csym = sym COMMON_LISP`;
+val ksym_def = Define `ksym = sym KEYWORD`;
+val osym_def = Define `osym = sym ACL2_OUTPUT_CHANNEL`;
+
+val let_simp =
+ prove
+  (``!P v y. (let (x,y) = (v,y) in P x y) = (let x = v in P x y)``,
+   RW_TAC std_ss []
+    THEN FULL_SIMP_TAC std_ss [markerTheory.Abbrev_def]);
+
+val simp_defs = let_simp 
+                :: map GSYM [int_def,nat_def,
+                             List_def, acl2_and_def,
+                             acl2_and_def,
+                             asym_def,csym_def,ksym_def,osym_def];
+
+val simp_defaxioms = ref([] : thm list);
+
+simp_defaxioms := time (map(SIMP_RULE std_ss simp_defs)) (!defaxioms);
+
+val abbrev_thms = 
+ CONJUNCT1 List_def :: CONJUNCT1 acl2_and_def :: string_abbrev_thms;
+
+simp_defaxioms := time (map (SUBS abbrev_thms)) (!simp_defaxioms);
+
+!simp_defaxioms;
+
+(*
+val _ = export_acl2_theory();
+*)
 
